pulse/src/checker/Pulse.Checker.Rewrite.fst
@@ -25,6 +25,7 @@ open Pulse.Checker.ImpureSpec
 open Pulse.PP
 module T = FStar.Tactics.V2
 module R = FStar.Reflection.V2
+module RTS = FStar.Reflection.TermSpec
 module RU = Pulse.RuntimeUtils
 
 let check_slprop_equiv_ext r (g:env) (p q:slprop)
@@ -58,7 +59,7 @@ let check_slprop_equiv_tac r (g:env) (p q:slprop) (tac_tm : term)
   let goal = Pulse.Reflection.Util.stt_slprop_equiv p q in
   let goal = mk_squash goal in
   let r_env = elab_env g in
-  let goal_typing_tok : squash (T.typing_token r_env goal (E_Total, R.pack_ln (R.Tv_Type u0))) =
+  let goal_typing_tok : squash (T.typing_token r_env (RTS.denote_term goal) (E_Total, RTS.denote_term (R.pack_ln (R.Tv_Type u0)))) =
     RU.magic ()
   in
   let res, issues = T.call_subtac_tm r_env tac_tm u0 goal in
