pulse/src/checker/Pulse.Elaborate.Pure.fst
@@ -16,6 +16,7 @@
 
 module Pulse.Elaborate.Pure
 module RT = FStar.Reflection.Typing
+module RTS = FStar.Reflection.TermSpec
 module R = FStar.Reflection.V2
 module L = FStar.List.Tot
 open FStar.List.Tot
@@ -96,16 +97,16 @@ let elab_comp (c:comp)
       mk_stt_ghost_comp u res inames pre (mk_abs res R.Q_Explicit post)
 
 let elab_stt_equiv (g:R.env) (c:comp{C_ST? c}) (pre:R.term) (post:R.term)
-  (eq_pre:RT.equiv g pre (comp_pre c))
-  (eq_post:RT.equiv g post
-                      (mk_abs (comp_res c) R.Q_Explicit (comp_post c)))
+  (eq_pre:RT.equiv g (RTS.denote_term pre) (RTS.denote_term (comp_pre c)))
+  (eq_post:RT.equiv g (RTS.denote_term post)
+                      (RTS.denote_term (mk_abs (comp_res c) R.Q_Explicit (comp_post c))))
   : RT.equiv g
-      (let C_ST {u;res} = c in
+      (RTS.denote_term (let C_ST {u;res} = c in
        mk_stt_comp u
                    res
                    pre
-                   post)
-      (elab_comp c) =
+                   post))
+      (RTS.denote_term (elab_comp c)) =
   
   mk_stt_comp_equiv _
     (comp_u c)
@@ -113,33 +114,33 @@ let elab_stt_equiv (g:R.env) (c:comp{C_ST? c}) (pre:R.term) (post:R.term)
     _ _ _ _ _ (RT.Rel_refl _ _ _) eq_pre eq_post
 
 let elab_stt_div_equiv (g:R.env) (c:comp{C_STDiv? c}) (pre:R.term) (post:R.term)
-  (eq_pre:RT.equiv g pre (comp_pre c))
-  (eq_post:RT.equiv g post
-                      (mk_abs (comp_res c) R.Q_Explicit (comp_post c)))
+  (eq_pre:RT.equiv g (RTS.denote_term pre) (RTS.denote_term (comp_pre c)))
+  (eq_post:RT.equiv g (RTS.denote_term post)
+                      (RTS.denote_term (mk_abs (comp_res c) R.Q_Explicit (comp_post c))))
   : RT.equiv g
-      (let C_STDiv {u;res} = c in
+      (RTS.denote_term (let C_STDiv {u;res} = c in
        mk_stt_div_comp u
                    res
                    pre
-                   post)
-      (elab_comp c) =
+                   post))
+      (RTS.denote_term (elab_comp c)) =
 
   mk_stt_div_comp_equiv _
     (comp_u c)
     (comp_res c)
     _ _ _ _ _ (RT.Rel_refl _ _ _) eq_pre eq_post
 let elab_statomic_equiv (g:R.env) (c:comp{C_STAtomic? c}) (pre:R.term) (post:R.term)
-  (eq_pre:RT.equiv g pre (comp_pre c))
-  (eq_post:RT.equiv g post
-                    (mk_abs (comp_res c) R.Q_Explicit (comp_post c)))
+  (eq_pre:RT.equiv g (RTS.denote_term pre) (RTS.denote_term (comp_pre c)))
+  (eq_post:RT.equiv g (RTS.denote_term post)
+                    (RTS.denote_term (mk_abs (comp_res c) R.Q_Explicit (comp_post c))))
   : RT.equiv g
-      (let C_STAtomic inames obs {u;res} = c in
+      (RTS.denote_term (let C_STAtomic inames obs {u;res} = c in
        mk_stt_atomic_comp (elab_observability obs) u
                           res
                           inames
                           pre
-                          post)
-      (elab_comp c) =
+                          post))
+      (RTS.denote_term (elab_comp c)) =
   
   let C_STAtomic inames obs {u;res} = c in
   let c' =
@@ -156,17 +157,17 @@ let elab_statomic_equiv (g:R.env) (c:comp{C_STAtomic? c}) (pre:R.term) (post:R.t
       _ _ _ _ eq_pre eq_post
 
 let elab_stghost_equiv (g:R.env) (c:comp{C_STGhost? c}) (pre:R.term) (post:R.term)
-  (eq_pre:RT.equiv g pre (comp_pre c))
-  (eq_post:RT.equiv g post
-                    (mk_abs (comp_res c) R.Q_Explicit (comp_post c)))
+  (eq_pre:RT.equiv g (RTS.denote_term pre) (RTS.denote_term (comp_pre c)))
+  (eq_post:RT.equiv g (RTS.denote_term post)
+                    (RTS.denote_term (mk_abs (comp_res c) R.Q_Explicit (comp_post c))))
   : RT.equiv g
-      (let C_STGhost inames {u;res} = c in
+      (RTS.denote_term (let C_STGhost inames {u;res} = c in
        mk_stt_ghost_comp u
                          res
                          inames
                          pre
-                         post)
-      (elab_comp c) =
+                         post))
+      (RTS.denote_term (elab_comp c)) =
   
   let C_STGhost inames _ = c in
   mk_stt_ghost_comp_equiv _
