pulse/src/checker/Pulse.Main.fst
@@ -19,6 +19,7 @@ module Pulse.Main
 module T = FStar.Tactics.V2
 module R = FStar.Reflection.V2
 module RT = FStar.Reflection.Typing
+module RTS = FStar.Reflection.TermSpec
 open FStar.Tactics.V2
 
 open Pulse.Syntax
@@ -148,7 +149,7 @@ let check_fndefn
 
   let mk_main_decl
     (refl_t:typ)
-    (_:squash (Nonempty.nonempty (RT.tot_typing (elab_env g) (RU.magic #R.term ()) refl_t))) =
+    (_:squash (Nonempty.nonempty (RT.tot_typing (elab_env g) (RTS.denote_term (RU.magic #R.term ())) (RTS.denote_term refl_t)))) =
     let nm = fst (inspect_ident id) in
     Reflection.Util.mk_opaque_let (fstar_env g) cur_module nm us (RU.magic #R.term ()) refl_t
   in
