pulse/src/checker/Pulse.Typing.Util.fsti
@@ -17,20 +17,21 @@
 module Pulse.Typing.Util
 
 open FStar.Tactics.V2
+module RTS = FStar.Reflection.TermSpec
 
 (* Like T.check_equiv, but will make sure to not delay any VC. *)
 val check_equiv_now (g:env) (t1 t2 : term)
-  : Tac (option (squash (equiv_token g t1 t2)) & issues)
+  : Tac (option (squash (equiv_token g (RTS.denote_term t1) (RTS.denote_term t2))) & issues)
 
 (* As above, but disallowing SMT (and unfolding). This is supposed
 to be a rather fast, unification-only check. *)
 val check_equiv_now_nosmt (g:env) (t1 t2 : term)
-  : Tac (option (squash (equiv_token g t1 t2)) & issues)
+  : Tac (option (squash (equiv_token g (RTS.denote_term t1) (RTS.denote_term t2))) & issues)
 
 (* As above, but allowing unfolding. *)
 val check_equiv_now_nosmt_unfold (g:env) (t1 t2 : term)
-  : Tac (option (squash (equiv_token g t1 t2)) & issues)
+  : Tac (option (squash (equiv_token g (RTS.denote_term t1) (RTS.denote_term t2))) & issues)
 
 (* Like T.universe_of, but will make sure to not delay any VC. *)
 val universe_of_now : g:env -> e:term ->
-  Tac (option (u:universe{typing_token g e (E_Total, pack_ln (Reflection.V2.Tv_Type u))}) & issues)
+  Tac (option (u:universe{typing_token g (RTS.denote_term e) (E_Total, RTS.Ts_Type (RTS.denote_universe u))}) & issues)
